\documentclass{article}
\usepackage{fullpage}
\usepackage[utf8x]{inputenc}
\usepackage{amssymb}
\usepackage{amsthm}
\usepackage{amsmath}
\usepackage{hyperref}
\usepackage{cleveref}
\usepackage{autonum}
\usepackage{dsfont}
\usepackage{stmaryrd}

\newtheorem{theorem}{Theorem}
\newtheorem{lemma}{Lemma}
\newtheorem{remark}{Remark}
\newtheorem{corollary}{Corollary}



\author{Bruno Scherrer}
\def\R{\mathds R}
\def\1{{\mathds 1}}

\newcommand{\intset}[1]{\llbracket #1 \rrbracket}
\newcommand{\intpart}[1]{\lceil #1 \rceil}

\begin{document}

For any policy $\vec\mu=\mu_1,\dots,\mu_n$, for any state $x$ and any stationary adversary policy $\nu$, there exists a decomposition:
\begin{align}
\vec\mu = \vec\mu_P \vec\mu_C \vec\mu_{P'}
\end{align}
such that
\begin{align}
  \1_x P_{\vec\mu_P,\nu} = \1_x P_{\vec\mu_P,\nu} P_{\vec\mu_C,\nu} = \1_y(\vec\mu,x,\nu)
\end{align}
If we consider the policy $\tilde \mu(\vec\mu,x,\nu) = \mu_P (\mu_C)^\infty$, then for any $w$,
\begin{align}
  v_{\tilde\mu(\vec\mu,x,\nu),\nu}(x) - T_{\vec\mu_P,\nu}T_{\vec\mu_C,\nu} w(x) &= \1_x[  T_{\vec\mu_P,\nu} (T_{\vec\mu_C,\nu})^{\infty}w  - T_{\vec\mu_P,\nu}T_{\vec\mu_C,\nu} w] \\
  & = \sum_{k=1}^\infty \1_x T_{\vec\mu_P,\nu} (T_{\vec\mu_C,\nu})^{k+1} w - \1_x T_{\vec\mu_P,\nu} (T_{\vec\mu_C,\nu})^{k} w \\
  & =  \sum_{k=1}^\infty \1_x \Gamma_{\vec\mu_P,\nu} (\Gamma_{\vec\mu_C,\nu})^k (T_{\vec\mu_C,\nu} w - w) \\
  & = \frac{\gamma^{i+c}}{1-\gamma^c} \1_{y(\vec\mu,x,\nu)}  (T_{\vec\mu_C,\nu} w - w).
\end{align}
Therefore by taking $w=T_{\vec\mu_{P'},\nu} v$, we get for any $v$, 
\begin{align}
  v_{\tilde\mu(\vec\mu,x,\nu),\nu}(x) - T_{\vec\mu,\nu} v(x) = \frac{\gamma^{i+c}}{1-\gamma^c} \1_{y(\vec\mu,x,\nu)}  (T_{\vec\mu_C,\nu}T_{\vec\mu_{P'},\nu} v  - T_{\vec\mu_{P'},\nu} v).
\end{align}

Symmetrically we have for any policy $\vec\nu=\nu_1 \dots \nu_n$, any state $x$ and any stationary adversary policy $\mu$, 
\begin{align}
 v_{\mu,\tilde\nu(\vec\nu,x,\mu)}(x) - T_{\mu,\vec\nu} v(x) = \frac{\gamma^{j+d}}{1-\gamma^d} \1_{z(\vec\nu,x,\mu)}  (T_{\mu,\vec\nu_C}T_{\mu,\vec\nu_{P'}} v  - T_{\mu,\vec\nu_{P'}} v).
\end{align}

Assume $v \ge Tv$ and
\begin{align}
  T_{\mu_1,\nu_1} \dots T_{\mu_n,\nu_n}v = T_{\vec\mu,\vec\nu}v = T^n v. 
\end{align}
On the one hand, we have
\begin{align}
  v_{\mu_*,\nu_*}(x)-T^n v(x) &\le v_{\mu_*,\tilde\nu(\vec\nu,x,\mu_*)}(x)-T^n v(x) \\
  & = \frac{\gamma^{j+d}}{1-\gamma^d} \1_{z(\vec\nu,x,\mu_*)}  (T_{\mu_*,\vec\nu_C}T_{\mu_*,\vec\nu_{P'}} v  - T_{\mu_*,\vec\nu_{P'}} v) \\
  & \le \frac{\gamma^{j+d}}{1-\gamma^d} \1_{z(\vec\nu,x,\mu_*)}  (T^{n-j-d}v -T^{n-j}v).
\end{align}
From $z$ such that $T^{n-j-d}v -T^{n-j}v \le \rho$, can we do $\vec\nu_C$ and then force any policy $\mu_*$ to revisit $z$ ? If yes, then we have a bound on $v_*$.


On the other hand, we have for all $\bar\nu$;
\begin{align}
  v_{\tilde\mu(\vec\mu,x,\bar\nu)}(x) - T^n v(x) & = \frac{\gamma^{i+c}}{1-\gamma^c} \1_{y(\vec\mu,x,\bar\nu)}  (T_{\vec\mu_C,\bar\nu}T_{\vec\mu_{P'},\bar\nu} v  - T_{\vec\mu_{P'},\bar\nu} v) \\
  & \ge  \frac{\gamma^{i+c}}{1-\gamma^c} \1_{y(\vec\mu,x,\bar\nu)}  (T^{n-i-c}v - T^{n-i}v).
\end{align}
From $y$, such that $T^{n-j-d}v -T^{n-j}v > \rho$, can we do $\vec\mu_C$ and then force any policy $\bar\nu$ to revisit $y$ ? If yes, then we make a significant improvement.




\bibliographystyle{plain}
\bibliography{biblio}


\end{document}


